test/Util/UTF8.dfy
@@ -5,7 +5,6 @@ include "../../src/StandardLibrary/StandardLibrary.dfy"
 include "../../src/Util/UTF8.dfy"
 
 module TestUTF8 {
-  import opened StandardLibrary
   import opened UInt = StandardLibrary.UInt
   import opened UTF8
 
